Sorting finished thanks to Dr.Tasistro.

code/dafny/sorting.dfy
@@ -4,82 +4,45 @@ predicate sorted(a: array<int>, low: int, high :int)
     requires 0 <= low <= high <= a.Length;
     reads a;
     {
-        forall j, k ::low <= j < k < high ==> a[j] <= a[k]
+        forall j, k :: low <= j < k < high ==> a[j] <= a[k]
     }
 
-
-// Swap two items from an array
-method swap<T>(a: array<T>, first: nat, second: nat)
+predicate leq_partitioned(a:array<int>, r:int)
+    reads a;
     requires a != null;
-    requires a.Length > 0;
-    requires 0 <= first < a.Length;
-    requires 0 <= second < a.Length;
-    modifies a;
-    ensures old(a.Length) == a.Length;
-    ensures old(a[first]) == a[second];
-    ensures old(a[second]) == a[first];
-    ensures forall m :: 0 <= m < a.Length && m != first
-                        && m != second ==> a[m] == old(a[m]);
-    ensures multiset(a[..]) == old(multiset(a[..]));
     {
-        // Init
-        a[first], a[second] := a[second], a[first];
+        forall j, k :: 0 <= j < r <= k < a.Length ==> a[j] <= a[k]
     }
 
-
-method swap_next(a: array<int>, index: int)
-    requires a != null;
-    requires a.Length > 1;
-    requires index + 1 < a.Length;
-    requires index >= 0;
-    ensures a[index] <= a[index + 1];
-    ensures multiset(a[..]) == old(multiset(a[..]));
-    //ensures sorted(a, index, index + 1);
+method bubble_sort(a:array<int>)
     modifies a;
-    {
-        if(a[index] > a[index + 1]){
-            swap(a, index, index + 1);
-        }
-    }
-
-
-method bubble_sort(a: array<int>)
     requires a != null;
-    modifies a;
     ensures multiset(a[..]) == old(multiset(a[..]));
-    //ensures sorted(a, 0, a.Length);
+    ensures sorted(a,0,a.Length)
     {
-        var r: int;
-        // Init
+        var r:int;
         r := a.Length;
-
-        while (r !=0 )
-        invariant 0 <= r <= a.Length;
+        while(r != 0)
+        invariant a.Length >= r >= 0;
         invariant multiset(a[..]) == old(multiset(a[..]));
-        invariant sorted(a, r, a.Length);
-        invariant forall j, k : int :: 0 <= j < r && r <= k < a.Length ==> a[j] <= a[k];
-        decreases r;
+        invariant sorted(a,r,a.Length);
+        invariant leq_partitioned(a,r);
         {
-            var i: int;
-            // Init
+            var i : int;
             i := 0;
-
-            while (i+1 != r)
+            while(i+1 != r)
             invariant 0 <= i < r;
-            invariant forall j : int :: 0 <= j < i ==> a[j] <= a[i];
-            //invariant multiset(a[..]) == old(multiset(a[..]));
-            //invariant sorted(a, r, a.Length);
-            //invariant sorted(a, i, i + 1);
-            decreases r - i;
+            invariant forall j :: 0 <= j < i ==> a[j] <= a[i];
+            invariant leq_partitioned(a,r);
+            invariant sorted(a,r,a.Length);
+            invariant multiset(a[..]) == old(multiset(a[..]));
             {
-                // Order element
-                swap_next(a, i);
-                // Loop increment
-                i := i + 1;
-            }
-            assert forall j : int :: 0 <= j < r-1 ==> a[j] <= a[r-1];
-            assert forall k : int :: r <= k < a.Length ==> a[r-1] <= a[k];
-            // Loop decrement
-            r := r - 1;
+                if(a[i] > a[i+1]) {
+                    a[i], a[i+1] := a[i+1], a[i];
+                }
+                else {}
+                i := i+1 ;
+            } 
+            r := r-1 ;
         }
     }
